theories/aps_plus_2/definition.v
@@ -15,135 +15,135 @@ Definition aps_plus_mapping :=
   gmap data_function data_function.
 Implicit Types ξ : aps_plus_mapping.
 
-Inductive aps_plus_dir ξ : data_expr → data_expr → Prop :=
-  | aps_plus_dir_val v :
-      aps_plus_dir ξ
+Inductive aps_plus_expr_dir ξ : data_expr → data_expr → Prop :=
+  | aps_plus_expr_dir_val v :
+      aps_plus_expr_dir ξ
         v
         v
-  | aps_plus_dir_var x :
-      aps_plus_dir ξ
+  | aps_plus_expr_dir_var x :
+      aps_plus_expr_dir ξ
         $x
         $x
-  | aps_plus_dir_let eₛ1 eₛ2 eₜ1 eₜ2 :
-      aps_plus_dir ξ eₛ1 eₜ1 →
-      aps_plus_dir ξ eₛ2 eₜ2 →
-      aps_plus_dir ξ
+  | aps_plus_expr_dir_let eₛ1 eₛ2 eₜ1 eₜ2 :
+      aps_plus_expr_dir ξ eₛ1 eₜ1 →
+      aps_plus_expr_dir ξ eₛ2 eₜ2 →
+      aps_plus_expr_dir ξ
         (let: eₛ1 in eₛ2)
         (let: eₜ1 in eₜ2)
-  | aps_plus_dir_call eₛ1 eₛ2 eₜ1 eₜ2 :
-      aps_plus_dir ξ eₛ1 eₜ1 →
-      aps_plus_dir ξ eₛ2 eₜ2 →
-      aps_plus_dir ξ
+  | aps_plus_expr_dir_call eₛ1 eₛ2 eₜ1 eₜ2 :
+      aps_plus_expr_dir ξ eₛ1 eₜ1 →
+      aps_plus_expr_dir ξ eₛ2 eₜ2 →
+      aps_plus_expr_dir ξ
         (eₛ1 eₛ2)
         (eₜ1 eₜ2)
-  | aps_plus_dir_unop op eₛ eₜ :
-      aps_plus_dir ξ eₛ eₜ →
-      aps_plus_dir ξ
+  | aps_plus_expr_dir_unop op eₛ eₜ :
+      aps_plus_expr_dir ξ eₛ eₜ →
+      aps_plus_expr_dir ξ
         (DataUnop op eₛ)
         (DataUnop op eₜ)
-  | aps_plus_dir_binop op eₛ1 eₛ2 eₜ1 eₜ2 :
-      aps_plus_dir ξ eₛ1 eₜ1 →
-      aps_plus_dir ξ eₛ2 eₜ2 →
-      aps_plus_dir ξ
+  | aps_plus_expr_dir_binop op eₛ1 eₛ2 eₜ1 eₜ2 :
+      aps_plus_expr_dir ξ eₛ1 eₜ1 →
+      aps_plus_expr_dir ξ eₛ2 eₜ2 →
+      aps_plus_expr_dir ξ
         (DataBinop op eₛ1 eₛ2)
         (DataBinop op eₜ1 eₜ2)
-  | aps_plus_dir_plus_1 eₛ1 eₛ2 eₜ1 eₜ2 :
-      aps_plus_dir ξ eₛ1 eₜ1 →
-      aps_plus_aps ξ $0 eₛ2.[ren (+1)] eₜ2 →
-      aps_plus_dir ξ
+  | aps_plus_expr_dir_plus_1 eₛ1 eₛ2 eₜ1 eₜ2 :
+      aps_plus_expr_dir ξ eₛ1 eₜ1 →
+      aps_plus_expr_aps ξ $0 eₛ2.[ren (+1)] eₜ2 →
+      aps_plus_expr_dir ξ
         (eₛ1 + eₛ2)
         (let: eₜ1 in eₜ2)
-  | aps_plus_dir_plus_2 eₛ1 eₛ2 eₜ1 eₜ2 :
-      aps_plus_dir ξ eₛ2 eₜ2 →
-      aps_plus_aps ξ $0 eₛ1.[ren (+1)] eₜ1 →
-      aps_plus_dir ξ
+  | aps_plus_expr_dir_plus_2 eₛ1 eₛ2 eₜ1 eₜ2 :
+      aps_plus_expr_dir ξ eₛ2 eₜ2 →
+      aps_plus_expr_aps ξ $0 eₛ1.[ren (+1)] eₜ1 →
+      aps_plus_expr_dir ξ
         (eₛ1 + eₛ2)
         (let: eₜ2 in eₜ1)
-  | aps_plus_dir_binop_det op eₛ1 eₛ2 eₜ1 eₜ2 :
-      aps_plus_dir ξ eₛ1 eₜ1 →
-      aps_plus_dir ξ eₛ2 eₜ2 →
-      aps_plus_dir ξ
+  | aps_plus_expr_dir_binop_det op eₛ1 eₛ2 eₜ1 eₜ2 :
+      aps_plus_expr_dir ξ eₛ1 eₜ1 →
+      aps_plus_expr_dir ξ eₛ2 eₜ2 →
+      aps_plus_expr_dir ξ
         (DataBinopDet op eₛ1 eₛ2)
         (DataBinopDet op eₜ1 eₜ2)
-  | aps_plus_dir_if eₛ0 eₛ1 eₛ2 eₜ0 eₜ1 eₜ2 :
-      aps_plus_dir ξ eₛ0 eₜ0 →
-      aps_plus_dir ξ eₛ1 eₜ1 →
-      aps_plus_dir ξ eₛ2 eₜ2 →
-      aps_plus_dir ξ
+  | aps_plus_expr_dir_if eₛ0 eₛ1 eₛ2 eₜ0 eₜ1 eₜ2 :
+      aps_plus_expr_dir ξ eₛ0 eₜ0 →
+      aps_plus_expr_dir ξ eₛ1 eₜ1 →
+      aps_plus_expr_dir ξ eₛ2 eₜ2 →
+      aps_plus_expr_dir ξ
         (if: eₛ0 then eₛ1 else eₛ2)
         (if: eₜ0 then eₜ1 else eₜ2)
-  | aps_plus_dir_constr tag eₛ1 eₛ2 eₜ1 eₜ2 :
-      aps_plus_dir ξ eₛ1 eₜ1 →
-      aps_plus_dir ξ eₛ2 eₜ2 →
-      aps_plus_dir ξ
+  | aps_plus_expr_dir_constr tag eₛ1 eₛ2 eₜ1 eₜ2 :
+      aps_plus_expr_dir ξ eₛ1 eₜ1 →
+      aps_plus_expr_dir ξ eₛ2 eₜ2 →
+      aps_plus_expr_dir ξ
         (&tag eₛ1 eₛ2)
         (&tag eₜ1 eₜ2)
-  | aps_plus_dir_constr_det tag eₛ1 eₛ2 eₜ1 eₜ2 :
-      aps_plus_dir ξ eₛ1 eₜ1 →
-      aps_plus_dir ξ eₛ2 eₜ2 →
-      aps_plus_dir ξ
+  | aps_plus_expr_dir_constr_det tag eₛ1 eₛ2 eₜ1 eₜ2 :
+      aps_plus_expr_dir ξ eₛ1 eₜ1 →
+      aps_plus_expr_dir ξ eₛ2 eₜ2 →
+      aps_plus_expr_dir ξ
         (&&tag eₛ1 eₛ2)
         (&&tag eₜ1 eₜ2)
-  | aps_plus_dir_load eₛ1 eₛ2 eₜ1 eₜ2 :
-      aps_plus_dir ξ eₛ1 eₜ1 →
-      aps_plus_dir ξ eₛ2 eₜ2 →
-      aps_plus_dir ξ
+  | aps_plus_expr_dir_load eₛ1 eₛ2 eₜ1 eₜ2 :
+      aps_plus_expr_dir ξ eₛ1 eₜ1 →
+      aps_plus_expr_dir ξ eₛ2 eₜ2 →
+      aps_plus_expr_dir ξ
         (![eₛ2] eₛ1)
         (![eₜ2] eₜ1)
-  | aps_plus_dir_store eₛ1 eₛ2 eₛ3 eₜ1 eₜ2 eₜ3 :
-      aps_plus_dir ξ eₛ1 eₜ1 →
-      aps_plus_dir ξ eₛ2 eₜ2 →
-      aps_plus_dir ξ eₛ3 eₜ3 →
-      aps_plus_dir ξ
+  | aps_plus_expr_dir_store eₛ1 eₛ2 eₛ3 eₜ1 eₜ2 eₜ3 :
+      aps_plus_expr_dir ξ eₛ1 eₜ1 →
+      aps_plus_expr_dir ξ eₛ2 eₜ2 →
+      aps_plus_expr_dir ξ eₛ3 eₜ3 →
+      aps_plus_expr_dir ξ
         (eₛ1 <-[eₛ2]- eₛ3)
         (eₜ1 <-[eₜ2]- eₜ3)
-with aps_plus_aps ξ : data_expr → data_expr → data_expr → Prop :=
-  | aps_plus_aps_base acc eₛ eₜ :
-      aps_plus_dir ξ eₛ eₜ →
-      aps_plus_aps ξ acc
+with aps_plus_expr_aps ξ : data_expr → data_expr → data_expr → Prop :=
+  | aps_plus_expr_aps_base acc eₛ eₜ :
+      aps_plus_expr_dir ξ eₛ eₜ →
+      aps_plus_expr_aps ξ acc
         eₛ
         (eₜ + acc)
-  | aps_plus_aps_let acc eₛ1 eₛ2 eₜ1 eₜ2 :
-      aps_plus_dir ξ eₛ1 eₜ1 →
-      aps_plus_aps ξ acc.[ren (+1)] eₛ2 eₜ2 →
-      aps_plus_aps ξ acc
+  | aps_plus_expr_aps_let acc eₛ1 eₛ2 eₜ1 eₜ2 :
+      aps_plus_expr_dir ξ eₛ1 eₜ1 →
+      aps_plus_expr_aps ξ acc.[ren (+1)] eₛ2 eₜ2 →
+      aps_plus_expr_aps ξ acc
         (let: eₛ1 in eₛ2)
         (let: eₜ1 in eₜ2)
-  | aps_plus_aps_call acc func annot eₛ func_aps eₜ eₜ' :
+  | aps_plus_expr_aps_call acc func annot eₛ func_aps eₜ eₜ' :
       ξ !! func = Some func_aps →
-      aps_plus_dir ξ eₛ eₜ →
+      aps_plus_expr_dir ξ eₛ eₜ →
       eₜ' = (let: eₜ in (DataFunc func_aps annot) (acc.[ren (+1)], $0))%data_expr →
-      aps_plus_aps ξ acc
+      aps_plus_expr_aps ξ acc
         ((DataFunc func annot) eₛ)
         eₜ'
-  | aps_plus_aps_plus_1 acc eₛ1 eₛ2 eₜ1 eₜ2 :
-      aps_plus_dir ξ eₛ1 eₜ1 →
-      aps_plus_aps ξ $0 eₛ2.[ren (+1)] eₜ2 →
-      aps_plus_aps ξ acc
+  | aps_plus_expr_aps_plus_1 acc eₛ1 eₛ2 eₜ1 eₜ2 :
+      aps_plus_expr_dir ξ eₛ1 eₜ1 →
+      aps_plus_expr_aps ξ $0 eₛ2.[ren (+1)] eₜ2 →
+      aps_plus_expr_aps ξ acc
         (eₛ1 + eₛ2)
         (let: eₜ1 + acc in eₜ2)
-  | aps_plus_aps_plus_2 acc eₛ1 eₛ2 eₜ1 eₜ2 :
-      aps_plus_dir ξ eₛ2 eₜ2 →
-      aps_plus_aps ξ $0 eₛ1.[ren (+1)] eₜ1 →
-      aps_plus_aps ξ acc
+  | aps_plus_expr_aps_plus_2 acc eₛ1 eₛ2 eₜ1 eₜ2 :
+      aps_plus_expr_dir ξ eₛ2 eₜ2 →
+      aps_plus_expr_aps ξ $0 eₛ1.[ren (+1)] eₜ1 →
+      aps_plus_expr_aps ξ acc
         (eₛ1 + eₛ2)
         (let: eₜ2 + acc in eₜ1)
-  | aps_plus_aps_if acc eₛ0 eₛ1 eₛ2 eₜ0 eₜ1 eₜ2 :
-      aps_plus_dir ξ eₛ0 eₜ0 →
-      aps_plus_aps ξ acc eₛ1 eₜ1 →
-      aps_plus_aps ξ acc eₛ2 eₜ2 →
-      aps_plus_aps ξ acc
+  | aps_plus_expr_aps_if acc eₛ0 eₛ1 eₛ2 eₜ0 eₜ1 eₜ2 :
+      aps_plus_expr_dir ξ eₛ0 eₜ0 →
+      aps_plus_expr_aps ξ acc eₛ1 eₜ1 →
+      aps_plus_expr_aps ξ acc eₛ2 eₜ2 →
+      aps_plus_expr_aps ξ acc
         (if: eₛ0 then eₛ1 else eₛ2)
         (if: eₜ0 then eₜ1 else eₜ2).
 
-Scheme aps_plus_dir_aps_ind := Minimality for aps_plus_dir Sort Prop
-with aps_plus_aps_dir_ind := Minimality for aps_plus_aps Sort Prop.
-Combined Scheme aps_plus_ind from aps_plus_dir_aps_ind, aps_plus_aps_dir_ind.
+Scheme aps_plus_expr_dir_aps_ind := Minimality for aps_plus_expr_dir Sort Prop
+with aps_plus_expr_aps_dir_ind := Minimality for aps_plus_expr_aps Sort Prop.
+Combined Scheme aps_plus_expr_ind from aps_plus_expr_dir_aps_ind, aps_plus_expr_aps_dir_ind.
 
 Create HintDb aps_plus.
 
-#[global] Hint Constructors aps_plus_dir : aps_plus.
-#[global] Hint Constructors aps_plus_aps : aps_plus.
+#[global] Hint Constructors aps_plus_expr_dir : aps_plus.
+#[global] Hint Constructors aps_plus_expr_aps : aps_plus.
 
 Record aps_plus {progₛ progₜ} := {
   aps_plus_ξ : gmap data_function data_function ;
@@ -153,11 +153,11 @@ Record aps_plus {progₛ progₜ} := {
   aps_plus_dom :
     dom progₜ = dom progₛ ∪ map_img aps_plus_ξ ;
 
-  aps_plus_dirs func defₛ eₛ :
+  aps_plus_dir func defₛ eₛ :
     progₛ !! func = Some defₛ →
     eₛ = defₛ.(data_definition_body) →
       ∃ eₜ,
-      aps_plus_dir aps_plus_ξ eₛ eₜ ∧
+      aps_plus_expr_dir aps_plus_ξ eₛ eₜ ∧
       progₜ !! func =
         Some {|
           data_definition_annot :=
@@ -166,12 +166,12 @@ Record aps_plus {progₛ progₜ} := {
             eₜ ;
         |} ;
 
-  aps_plus_apss func defₛ eₛ func_aps :
+  aps_plus_aps func defₛ eₛ func_aps :
     progₛ !! func = Some defₛ →
     eₛ = defₛ.(data_definition_body) →
     aps_plus_ξ !! func = Some func_aps →
       ∃ eₜ,
-      aps_plus_aps aps_plus_ξ $1 eₛ eₜ ∧
+      aps_plus_expr_aps aps_plus_ξ $1 eₛ eₜ ∧
       progₜ !! func_aps =
         Some {|
           data_definition_annot :=
