theories/tmc/definition.v
@@ -15,137 +15,137 @@ Definition tmc_mapping :=
   gmap data_function data_function.
 Implicit Types ξ : tmc_mapping.
 
-Inductive tmc_dir ξ : data_expr → data_expr → Prop :=
-  | tmc_dir_val v :
-      tmc_dir ξ
+Inductive tmc_expr_dir ξ : data_expr → data_expr → Prop :=
+  | tmc_expr_dir_val v :
+      tmc_expr_dir ξ
         v
         v
-  | tmc_dir_var x :
-      tmc_dir ξ
+  | tmc_expr_dir_var x :
+      tmc_expr_dir ξ
         $x
         $x
-  | tmc_dir_let eₛ1 eₛ2 eₜ1 eₜ2 :
-      tmc_dir ξ eₛ1 eₜ1 →
-      tmc_dir ξ eₛ2 eₜ2 →
-      tmc_dir ξ
+  | tmc_expr_dir_let eₛ1 eₛ2 eₜ1 eₜ2 :
+      tmc_expr_dir ξ eₛ1 eₜ1 →
+      tmc_expr_dir ξ eₛ2 eₜ2 →
+      tmc_expr_dir ξ
         (let: eₛ1 in eₛ2)
         (let: eₜ1 in eₜ2)
-  | tmc_dir_call eₛ1 eₛ2 eₜ1 eₜ2 :
-      tmc_dir ξ eₛ1 eₜ1 →
-      tmc_dir ξ eₛ2 eₜ2 →
-      tmc_dir ξ
+  | tmc_expr_dir_call eₛ1 eₛ2 eₜ1 eₜ2 :
+      tmc_expr_dir ξ eₛ1 eₜ1 →
+      tmc_expr_dir ξ eₛ2 eₜ2 →
+      tmc_expr_dir ξ
         (eₛ1 eₛ2)
         (eₜ1 eₜ2)
-  | tmc_dir_unop op eₛ eₜ :
-      tmc_dir ξ eₛ eₜ →
-      tmc_dir ξ
+  | tmc_expr_dir_unop op eₛ eₜ :
+      tmc_expr_dir ξ eₛ eₜ →
+      tmc_expr_dir ξ
         (DataUnop op eₛ)
         (DataUnop op eₜ)
-  | tmc_dir_binop op eₛ1 eₛ2 eₜ1 eₜ2 :
-      tmc_dir ξ eₛ1 eₜ1 →
-      tmc_dir ξ eₛ2 eₜ2 →
-      tmc_dir ξ
+  | tmc_expr_dir_binop op eₛ1 eₛ2 eₜ1 eₜ2 :
+      tmc_expr_dir ξ eₛ1 eₜ1 →
+      tmc_expr_dir ξ eₛ2 eₜ2 →
+      tmc_expr_dir ξ
         (DataBinop op eₛ1 eₛ2)
         (DataBinop op eₜ1 eₜ2)
-  | tmc_dir_binop_det op eₛ1 eₛ2 eₜ1 eₜ2 :
-      tmc_dir ξ eₛ1 eₜ1 →
-      tmc_dir ξ eₛ2 eₜ2 →
-      tmc_dir ξ
+  | tmc_expr_dir_binop_det op eₛ1 eₛ2 eₜ1 eₜ2 :
+      tmc_expr_dir ξ eₛ1 eₜ1 →
+      tmc_expr_dir ξ eₛ2 eₜ2 →
+      tmc_expr_dir ξ
         (DataBinopDet op eₛ1 eₛ2)
         (DataBinopDet op eₜ1 eₜ2)
-  | tmc_dir_if eₛ0 eₛ1 eₛ2 eₜ0 eₜ1 eₜ2 :
-      tmc_dir ξ eₛ0 eₜ0 →
-      tmc_dir ξ eₛ1 eₜ1 →
-      tmc_dir ξ eₛ2 eₜ2 →
-      tmc_dir ξ
+  | tmc_expr_dir_if eₛ0 eₛ1 eₛ2 eₜ0 eₜ1 eₜ2 :
+      tmc_expr_dir ξ eₛ0 eₜ0 →
+      tmc_expr_dir ξ eₛ1 eₜ1 →
+      tmc_expr_dir ξ eₛ2 eₜ2 →
+      tmc_expr_dir ξ
         (if: eₛ0 then eₛ1 else eₛ2)
         (if: eₜ0 then eₜ1 else eₜ2)
-  | tmc_dir_constr tag eₛ1 eₛ2 eₜ1 eₜ2 :
-      tmc_dir ξ eₛ1 eₜ1 →
-      tmc_dir ξ eₛ2 eₜ2 →
-      tmc_dir ξ
+  | tmc_expr_dir_constr tag eₛ1 eₛ2 eₜ1 eₜ2 :
+      tmc_expr_dir ξ eₛ1 eₜ1 →
+      tmc_expr_dir ξ eₛ2 eₜ2 →
+      tmc_expr_dir ξ
         (&tag eₛ1 eₛ2)
         (&tag eₜ1 eₜ2)
-  | tmc_dir_constr_dps_1 tag eₛ1 eₛ2 eₜ1 eₜ2 :
-      tmc_dir ξ eₛ1 eₜ1 →
-      tmc_dps ξ $0 𝟚 eₛ2.[ren (+1)] eₜ2 →
-      tmc_dir ξ
+  | tmc_expr_dir_constr_dps_1 tag eₛ1 eₛ2 eₜ1 eₜ2 :
+      tmc_expr_dir ξ eₛ1 eₜ1 →
+      tmc_expr_dps ξ $0 𝟚 eₛ2.[ren (+1)] eₜ2 →
+      tmc_expr_dir ξ
         (&tag eₛ1 eₛ2)
         (let: &tag eₜ1 #() in eₜ2 ;; $0)
-  | tmc_dir_constr_dps_2 tag eₛ1 eₛ2 eₜ1 eₜ2 :
-      tmc_dir ξ eₛ2 eₜ2 →
-      tmc_dps ξ $0 𝟙 eₛ1.[ren (+1)] eₜ1 →
-      tmc_dir ξ
+  | tmc_expr_dir_constr_dps_2 tag eₛ1 eₛ2 eₜ1 eₜ2 :
+      tmc_expr_dir ξ eₛ2 eₜ2 →
+      tmc_expr_dps ξ $0 𝟙 eₛ1.[ren (+1)] eₜ1 →
+      tmc_expr_dir ξ
         (&tag eₛ1 eₛ2)
         (let: &tag #() eₜ2 in eₜ1 ;; $0)
-  | tmc_dir_constr_det tag eₛ1 eₛ2 eₜ1 eₜ2 :
-      tmc_dir ξ eₛ1 eₜ1 →
-      tmc_dir ξ eₛ2 eₜ2 →
-      tmc_dir ξ
+  | tmc_expr_dir_constr_det tag eₛ1 eₛ2 eₜ1 eₜ2 :
+      tmc_expr_dir ξ eₛ1 eₜ1 →
+      tmc_expr_dir ξ eₛ2 eₜ2 →
+      tmc_expr_dir ξ
         (&&tag eₛ1 eₛ2)
         (&&tag eₜ1 eₜ2)
-  | tmc_dir_load eₛ1 eₛ2 eₜ1 eₜ2 :
-      tmc_dir ξ eₛ1 eₜ1 →
-      tmc_dir ξ eₛ2 eₜ2 →
-      tmc_dir ξ
+  | tmc_expr_dir_load eₛ1 eₛ2 eₜ1 eₜ2 :
+      tmc_expr_dir ξ eₛ1 eₜ1 →
+      tmc_expr_dir ξ eₛ2 eₜ2 →
+      tmc_expr_dir ξ
         (![eₛ2] eₛ1)
         (![eₜ2] eₜ1)
-  | tmc_dir_store eₛ1 eₛ2 eₛ3 eₜ1 eₜ2 eₜ3 :
-      tmc_dir ξ eₛ1 eₜ1 →
-      tmc_dir ξ eₛ2 eₜ2 →
-      tmc_dir ξ eₛ3 eₜ3 →
-      tmc_dir ξ
+  | tmc_expr_dir_store eₛ1 eₛ2 eₛ3 eₜ1 eₜ2 eₜ3 :
+      tmc_expr_dir ξ eₛ1 eₜ1 →
+      tmc_expr_dir ξ eₛ2 eₜ2 →
+      tmc_expr_dir ξ eₛ3 eₜ3 →
+      tmc_expr_dir ξ
         (eₛ1 <-[eₛ2]- eₛ3)
         (eₜ1 <-[eₜ2]- eₜ3)
-with tmc_dps ξ : data_expr → data_expr → data_expr → data_expr → Prop :=
-  | tmc_dps_base dst idx eₛ eₜ :
-      tmc_dir ξ eₛ eₜ →
-      tmc_dps ξ dst idx
+with tmc_expr_dps ξ : data_expr → data_expr → data_expr → data_expr → Prop :=
+  | tmc_expr_dps_base dst idx eₛ eₜ :
+      tmc_expr_dir ξ eₛ eₜ →
+      tmc_expr_dps ξ dst idx
         eₛ
         (dst <-[idx]- eₜ)
-  | tmc_dps_let dst idx eₛ1 eₛ2 eₜ1 eₜ2 :
-      tmc_dir ξ eₛ1 eₜ1 →
-      tmc_dps ξ dst.[ren (+1)] idx.[ren (+1)] eₛ2 eₜ2 →
-      tmc_dps ξ dst idx
+  | tmc_expr_dps_let dst idx eₛ1 eₛ2 eₜ1 eₜ2 :
+      tmc_expr_dir ξ eₛ1 eₜ1 →
+      tmc_expr_dps ξ dst.[ren (+1)] idx.[ren (+1)] eₛ2 eₜ2 →
+      tmc_expr_dps ξ dst idx
         (let: eₛ1 in eₛ2)
         (let: eₜ1 in eₜ2)
-  | tmc_dps_call dst idx func annot eₛ func_dps eₜ eₜ' :
+  | tmc_expr_dps_call dst idx func annot eₛ func_dps eₜ eₜ' :
       ξ !! func = Some func_dps →
-      tmc_dir ξ eₛ eₜ →
+      tmc_expr_dir ξ eₛ eₜ →
       eₜ' = (let: eₜ in (DataFunc func_dps annot) (dst.[ren (+1)], idx.[ren (+1)], $0))%data_expr →
-      tmc_dps ξ dst idx
+      tmc_expr_dps ξ dst idx
         ((DataFunc func annot) eₛ)
         eₜ'
-  | tmc_dps_if dst idx eₛ0 eₛ1 eₛ2 eₜ0 eₜ1 eₜ2 :
-      tmc_dir ξ eₛ0 eₜ0 →
-      tmc_dps ξ dst idx eₛ1 eₜ1 →
-      tmc_dps ξ dst idx eₛ2 eₜ2 →
-      tmc_dps ξ dst idx
+  | tmc_expr_dps_if dst idx eₛ0 eₛ1 eₛ2 eₜ0 eₜ1 eₜ2 :
+      tmc_expr_dir ξ eₛ0 eₜ0 →
+      tmc_expr_dps ξ dst idx eₛ1 eₜ1 →
+      tmc_expr_dps ξ dst idx eₛ2 eₜ2 →
+      tmc_expr_dps ξ dst idx
         (if: eₛ0 then eₛ1 else eₛ2)
         (if: eₜ0 then eₜ1 else eₜ2)
-  | tmc_dps_constr_1 dst idx tag eₛ1 eₛ2 eₜ1 eₜ2 eₜ :
-      tmc_dir ξ eₛ1 eₜ1 →
-      tmc_dps ξ $0 𝟚 eₛ2.[ren (+1)] eₜ2 →
+  | tmc_expr_dps_constr_1 dst idx tag eₛ1 eₛ2 eₜ1 eₜ2 eₜ :
+      tmc_expr_dir ξ eₛ1 eₜ1 →
+      tmc_expr_dps ξ $0 𝟚 eₛ2.[ren (+1)] eₜ2 →
       eₜ = (let: &tag eₜ1 #() in dst.[ren (+1)] <-[idx.[ren (+1)]]- $0 ;; eₜ2)%data_expr →
-      tmc_dps ξ dst idx
+      tmc_expr_dps ξ dst idx
         (&tag eₛ1 eₛ2)
         eₜ
-  | tmc_dps_constr_2 dst idx tag eₛ1 eₛ2 eₜ1 eₜ2 eₜ :
-      tmc_dir ξ eₛ2 eₜ2 →
-      tmc_dps ξ $0 𝟙 eₛ1.[ren (+1)] eₜ1 →
+  | tmc_expr_dps_constr_2 dst idx tag eₛ1 eₛ2 eₜ1 eₜ2 eₜ :
+      tmc_expr_dir ξ eₛ2 eₜ2 →
+      tmc_expr_dps ξ $0 𝟙 eₛ1.[ren (+1)] eₜ1 →
       eₜ = (let: &tag #() eₜ2 in dst.[ren (+1)] <-[idx.[ren (+1)]]- $0 ;; eₜ1)%data_expr →
-      tmc_dps ξ dst idx
+      tmc_expr_dps ξ dst idx
         (&tag eₛ1 eₛ2)
         eₜ.
 
-Scheme tmc_dir_dps_ind := Minimality for tmc_dir Sort Prop
-with tmc_dps_dir_ind := Minimality for tmc_dps Sort Prop.
-Combined Scheme tmc_ind from tmc_dir_dps_ind, tmc_dps_dir_ind.
+Scheme tmc_expr_dir_dps_ind := Minimality for tmc_expr_dir Sort Prop
+with tmc_expr_dps_dir_ind := Minimality for tmc_expr_dps Sort Prop.
+Combined Scheme tmc_expr_ind from tmc_expr_dir_dps_ind, tmc_expr_dps_dir_ind.
 
 Create HintDb tmc.
 
-#[global] Hint Constructors tmc_dir : tmc.
-#[global] Hint Constructors tmc_dps : tmc.
+#[global] Hint Constructors tmc_expr_dir : tmc.
+#[global] Hint Constructors tmc_expr_dps : tmc.
 
 Record tmc {progₛ progₜ} := {
   tmc_ξ : gmap data_function data_function ;
@@ -155,11 +155,11 @@ Record tmc {progₛ progₜ} := {
   tmc_dom :
     dom progₜ = dom progₛ ∪ map_img tmc_ξ ;
 
-  tmc_dirs func defₛ eₛ :
+  tmc_dir func defₛ eₛ :
     progₛ !! func = Some defₛ →
     eₛ = defₛ.(data_definition_body) →
       ∃ eₜ,
-      tmc_dir tmc_ξ eₛ eₜ ∧
+      tmc_expr_dir tmc_ξ eₛ eₜ ∧
       progₜ !! func =
         Some {|
           data_definition_annot :=
@@ -168,12 +168,12 @@ Record tmc {progₛ progₜ} := {
             eₜ ;
         |} ;
 
-  tmc_dpss func defₛ eₛ func_dps :
+  tmc_dps func defₛ eₛ func_dps :
     progₛ !! func = Some defₛ →
     eₛ = defₛ.(data_definition_body) →
     tmc_ξ !! func = Some func_dps →
       ∃ eₜ,
-      tmc_dps tmc_ξ $1 $2 eₛ eₜ ∧
+      tmc_expr_dps tmc_ξ $1 $2 eₛ eₜ ∧
       progₜ !! func_dps =
         Some {|
           data_definition_annot :=
