theories/tmc/soundness.v
@@ -77,54 +77,54 @@ Section sim_GS.
       ).
   Qed.
 
-  Definition tmc_dir_post :=
+  Definition tmc_expr_dir_post :=
     (≈)%I.
-  Definition tmc_dps_post dst idx vₛ vₜ : iProp Σ :=
+  Definition tmc_expr_dps_post dst idx vₛ vₜ : iProp Σ :=
     ∃ vₜ',
     ⌜vₜ = ()%data_val⌝ ∗ (dst +ₗ idx) ↦ₜ vₜ' ∗ vₛ ≈ vₜ'.
 
-  Definition tmc_dir_spec' eₛ eₜ :=
+  Definition tmc_expr_dir_spec' eₛ eₜ :=
     data_expr_well_formed sim_progₛ eₛ →
-    {{{ True }}} eₛ ⩾ eₜ [[ tmc_protocol ]] {{{# tmc_dir_post }}}.
-  Definition tmc_dir_spec eₛ eₜ :=
-    tmc_dir tmc.(tmc_ξ) eₛ eₜ →
-    tmc_dir_spec' eₛ eₜ.
-  Definition tmc_dps_spec' dst idx eₛ eₜ :=
+    {{{ True }}} eₛ ⩾ eₜ [[ tmc_protocol ]] {{{# tmc_expr_dir_post }}}.
+  Definition tmc_expr_dir_spec eₛ eₜ :=
+    tmc_expr_dir tmc.(tmc_ξ) eₛ eₜ →
+    tmc_expr_dir_spec' eₛ eₜ.
+  Definition tmc_expr_dps_spec' dst idx eₛ eₜ :=
     data_expr_well_formed sim_progₛ eₛ →
-    {{{ (dst +ₗ idx) ↦ₜ () }}} eₛ ⩾ eₜ [[ tmc_protocol ]] {{{# tmc_dps_post dst idx }}}.
-  Definition tmc_dps_spec dst idx eₛ eₜ :=
-    tmc_dps tmc.(tmc_ξ) dst idx eₛ eₜ →
-    tmc_dps_spec' dst idx eₛ eₜ.
-  Definition tmc_spec eₛ eₜ :=
-    tmc_dir_spec eₛ eₜ ∧
-    ∀ dst idx, tmc_dps_spec dst idx eₛ eₜ.
+    {{{ (dst +ₗ idx) ↦ₜ () }}} eₛ ⩾ eₜ [[ tmc_protocol ]] {{{# tmc_expr_dps_post dst idx }}}.
+  Definition tmc_expr_dps_spec dst idx eₛ eₜ :=
+    tmc_expr_dps tmc.(tmc_ξ) dst idx eₛ eₜ →
+    tmc_expr_dps_spec' dst idx eₛ eₜ.
+  Definition tmc_expr_spec eₛ eₜ :=
+    tmc_expr_dir_spec eₛ eₜ ∧
+    ∀ dst idx, tmc_expr_dps_spec dst idx eₛ eₜ.
 
-  Lemma tmc_specification eₛ eₜ :
-    tmc_spec eₛ eₜ.
+  Lemma tmc_expr_specification eₛ eₜ :
+    tmc_expr_spec eₛ eₜ.
   Proof.
     revert eₜ. induction eₛ as [eₛ IHeₛ] using (well_founded_ind data_subexpr_wf).
     cut (
       ( ∀ eₛ eₜ,
-        tmc_dir tmc.(tmc_ξ) eₛ eₜ →
-        (∀ eₛ' eₜ', eₛ' ⊏ eₛ → tmc_dir_spec eₛ' eₜ') →
-        (∀ dst idx eₛ' eₜ', eₛ' ⊏ eₛ → tmc_dps_spec dst idx eₛ' eₜ') →
-        tmc_dir_spec' eₛ eₜ
+        tmc_expr_dir tmc.(tmc_ξ) eₛ eₜ →
+        (∀ eₛ' eₜ', eₛ' ⊏ eₛ → tmc_expr_dir_spec eₛ' eₜ') →
+        (∀ dst idx eₛ' eₜ', eₛ' ⊏ eₛ → tmc_expr_dps_spec dst idx eₛ' eₜ') →
+        tmc_expr_dir_spec' eₛ eₜ
       ) ∧ (
         ∀ (dst idx : data_expr) eₛ eₜ,
-        tmc_dps tmc.(tmc_ξ) dst idx eₛ eₜ →
-        (∀ eₛ' eₜ', eₛ' ⊏ eₛ → tmc_dir_spec eₛ' eₜ') →
-        (∀ dst idx eₛ' eₜ', eₛ' ⊏ eₛ → tmc_dps_spec dst idx eₛ' eₜ') →
+        tmc_expr_dps tmc.(tmc_ξ) dst idx eₛ eₜ →
+        (∀ eₛ' eₜ', eₛ' ⊏ eₛ → tmc_expr_dir_spec eₛ' eₜ') →
+        (∀ dst idx eₛ' eₜ', eₛ' ⊏ eₛ → tmc_expr_dps_spec dst idx eₛ' eₜ') →
         ∀ dst' idx',
         dst = dst' →
         idx = idx' →
-        tmc_dps_spec' dst' idx' eₛ eₜ
+        tmc_expr_dps_spec' dst' idx' eₛ eₜ
       )
     ). {
-      rewrite /tmc_spec /tmc_dir_spec /tmc_dps_spec.
+      rewrite /tmc_expr_spec /tmc_expr_dir_spec /tmc_expr_dps_spec.
       naive_solver.
     }
-    clear eₛ IHeₛ. apply tmc_ind;
-      rewrite /tmc_dir_spec' /tmc_dps_spec';
+    clear eₛ IHeₛ. apply tmc_expr_ind;
+      rewrite /tmc_expr_dir_spec' /tmc_expr_dps_spec';
       intros *;
       [ intros _ _
       | intros _ _
@@ -148,7 +148,7 @@ Section sim_GS.
       | intros Hdir2 _ Hdps1 _ -> IHdirₛ IHdpsₛ dst' idx' -> ->
       ];
       iIntros "%Hwf %Φ Hpre HΦ".
-    (* tmc_dir *)
+    (* tmc_expr_dir *)
     - iApply rsimv_val; [done | iSmash].
     - iApply rsimv_var. iSmash.
     - iApply rsimv_let;
@@ -156,7 +156,7 @@ Section sim_GS.
     - iApply rsimv_call;
         [iApply IHdirₛ; auto with data_lang.. |].
       iIntros "%func %annot %vₛ %vₜ %Hfunc #Hv".
-      pose (Ψ := sim_post_vals' tmc_dir_post).
+      pose (Ψ := sim_post_vals' tmc_expr_dir_post).
       iApply (sim_apply_protocol _ Ψ). iIntros "%σₛ %σₜ $ !>". iSplitR.
       { rewrite /Ψ /sim_post_vals'. iSmash. }
       iIntros "% % (%vₛ' & %vₜ' & (-> & ->) & HΨ)".
@@ -178,7 +178,7 @@ Section sim_GS.
       sim_apply (IHdpsₛ lₜ 𝟚 eₛ2 eₜ2.[#lₜ/] with "Hlₜ2 [Hlₜ0 Hlₜ1 HΦ]"); first 4 last.
       { autosubst. }
       { auto with data_lang. }
-      { eapply tmc_dps_subst; eauto; autosubst. }
+      { eapply tmc_expr_dps_subst; eauto; autosubst. }
       { auto with data_lang. }
       iIntros "%vₛ2 % (%vₜ2 & -> & Hlₜ2 & #Hv2)".
       sim_constr_detₛ as lₛ "Hlₛ0" "Hlₛ1" "Hlₛ2".
@@ -197,7 +197,7 @@ Section sim_GS.
       sim_apply (IHdpsₛ lₜ 𝟙 eₛ1 eₜ1.[#lₜ/] with "Hlₜ1 [Hlₜ0 Hlₜ2 HΦ]"); first 4 last.
       { autosubst. }
       { auto with data_lang. }
-      { eapply tmc_dps_subst; eauto; autosubst. }
+      { eapply tmc_expr_dps_subst; eauto; autosubst. }
       { auto with data_lang. }
       iIntros "%vₛ1 % (%vₜ1 & -> & Hlₜ1 & #Hv1)".
       sim_constr_detₛ as lₛ "Hlₛ0" "Hlₛ1" "Hlₛ2".
@@ -213,7 +213,7 @@ Section sim_GS.
        iApply IHdirₛ; auto with data_lang.
     - iApply rsimv_store; last iSmash;
         iApply IHdirₛ; auto with data_lang.
-    (* tmc_dps *)
+    (* tmc_expr_dps *)
     - iIntros "%Γ % % (-> & ->) #HΓ /=".
       sim_apply (IHdir with "[//] [Hpre HΦ]"); [done.. |].
       iIntros "%vₛ %vₜ #Hv".
@@ -237,7 +237,7 @@ Section sim_GS.
       sim_apply (IHdpsₛ lₜ 𝟚 eₛ2 eₜ2.[#lₜ/] with "Hlₜ2 [Hpre Hlₜ0 Hlₜ1 HΦ] [] HΓ"); first 4 last.
       { autosubst. }
       { auto with data_lang. }
-      { eapply tmc_dps_subst; eauto; autosubst. }
+      { eapply tmc_expr_dps_subst; eauto; autosubst. }
       { auto with data_lang. }
       iIntros "%vₛ2 % (%vₜ2 & -> & Hlₜ2 & #Hv2)".
       sim_constr_detₛ as lₛ "Hlₛ0" "Hlₛ1" "Hlₛ2".
@@ -257,7 +257,7 @@ Section sim_GS.
       sim_apply (IHdpsₛ lₜ 𝟙 eₛ1 eₜ1.[#lₜ/] with "Hlₜ1 [Hpre Hlₜ0 Hlₜ2 HΦ] [] HΓ"); first 4 last.
       { autosubst. }
       { auto with data_lang. }
-      { eapply tmc_dps_subst; eauto; autosubst. }
+      { eapply tmc_expr_dps_subst; eauto; autosubst. }
       { auto with data_lang. }
       iIntros "%vₛ1 % (%vₜ1 & -> & Hlₜ1 & #Hv1)".
       sim_constr_detₛ as lₛ "Hlₛ0" "Hlₛ1" "Hlₛ2".
@@ -269,15 +269,15 @@ Section sim_GS.
       sim_heap_bij_insert.
       iSmash.
   Qed.
-  Lemma tmc_dir_specification eₛ eₜ :
-    tmc_dir_spec eₛ eₜ.
+  Lemma tmc_expr_dir_specification eₛ eₜ :
+    tmc_expr_dir_spec eₛ eₜ.
   Proof.
-    eapply proj1, tmc_specification.
+    eapply proj1, tmc_expr_specification.
   Qed.
-  Lemma tmc_dps_specification dst idx eₛ eₜ :
-    tmc_dps_spec dst idx eₛ eₜ.
+  Lemma tmc_expr_dps_specification dst idx eₛ eₜ :
+    tmc_expr_dps_spec dst idx eₛ eₜ.
   Proof.
-    revert dst idx. eapply proj2, tmc_specification.
+    revert dst idx. eapply proj2, tmc_expr_specification.
   Qed.
 
   Lemma tmc_simv_close Φ eₛ eₜ :
@@ -291,11 +291,11 @@ Section sim_GS.
     - iDestruct "Hprotocol" as "(%func & %annot & %vₛ & %vₜ & %Hfuncₛ & (-> & ->) & #Hv & HΨ)".
       simpl in Hfuncₛ. apply lookup_lookup_total_dom in Hfuncₛ.
       set defₛ := _ !!! _ in Hfuncₛ. set eₛ := defₛ.(data_definition_body).
-      edestruct tmc.(tmc_dirs) as (eₜ & Hdir & Hfuncₜ); [done.. |].
+      edestruct tmc.(tmc_dir) as (eₜ & Hdir & Hfuncₜ); [done.. |].
       iExists _, _. iSplit; first eauto 10 with data_lang. sim_asimpl.
       erewrite (subst_data_program_scoped' ids inhabitant.ₛ# _ sim_progₛ); [| done..].
       erewrite (subst_data_program_scoped' ids inhabitant.ₜ# _ sim_progₜ); [| done..].
-      iDestruct (tmc_dir_specification $! tmc_dir_post with "[//] [] [//] []") as "Hsim"; eauto.
+      iDestruct (tmc_expr_dir_specification $! tmc_expr_dir_post with "[//] [] [//] []") as "Hsim"; eauto.
       + iApply (bisubst_cons_well_formed with "Hv").
         iApply bisubst_inhabitant_well_formed.
       + rewrite -bisubst_consₛ -bisubst_consₜ.
@@ -303,16 +303,16 @@ Section sim_GS.
     - iDestruct "Hprotocol" as "(%func & %annot & %vₛ & %func_dps & %l1 & %l2 & %dst & %idx & %vₜ & (%Hfuncₛ & %Hξ) & (-> & ->) & Hl11 & Hl12 & Hl21 & Hl22 & Hdst & #Hv & HΨ)".
       simpl in Hfuncₛ. apply lookup_lookup_total_dom in Hfuncₛ.
       set defₛ := _ !!! _ in Hfuncₛ. set eₛ := defₛ.(data_definition_body).
-      edestruct tmc.(tmc_dpss) as (eₜ & Hdps & Hfunc_dpsₜ); [done.. |].
+      edestruct tmc.(tmc_dps) as (eₜ & Hdps & Hfunc_dpsₜ); [done.. |].
       iExists _, _. iSplit; first eauto 10 with data_lang. sim_asimpl.
       do 4 sim_loadₜ. sim_pures.
-      eapply (tmc_dps_subst _ (ids 0 .: #dst .: #idx .: ren (+1))) in Hdps; [| autosubst..].
+      eapply (tmc_expr_dps_subst _ (ids 0 .: #dst .: #idx .: ren (+1))) in Hdps; [| autosubst..].
       erewrite (subst_data_program_scoped' _ (ren (+1)) _ sim_progₛ) in Hdps; [| done..]. asimpl in Hdps.
       replace eₜ.[#vₜ, #dst, #idx, #l2, #l1/] with eₜ.[ids 0 .: #dst .: #idx .: ren (+1)].[#vₜ, #l2, #l1/] by autosubst.
       erewrite (subst_data_program_scoped' ids inhabitant.ₛ# _ sim_progₛ); [| done..].
       erewrite (subst_data_expr_scoped_1' (#l2 .: #l1 .: ids) inhabitant.ₜ#); last first.
-      { eapply data_expr_scoped_tmc_dps; naive_solver. }
-      iDestruct (tmc_dps_specification $! (tmc_dps_post dst idx) with "Hdst [] [//] []") as "Hsim"; eauto.
+      { eapply data_expr_scoped_tmc_expr_dps; naive_solver. }
+      iDestruct (tmc_expr_dps_specification $! (tmc_expr_dps_post dst idx) with "Hdst [] [//] []") as "Hsim"; eauto.
       + iApply (bisubst_cons_well_formed with "Hv").
         iApply bisubst_inhabitant_well_formed.
       + rewrite -bisubst_consₛ -bisubst_consₜ. asimpl.
