theories/tmc/examples/list_append.v
@@ -88,7 +88,7 @@ Proof.
       eexists. split; last done. repeat econstructor.
     + intros * (<- & <-)%lookup_singleton_Some -> (_ & <-)%lookup_singleton_Some.
       eexists. split; last done. repeat constructor.
-      eapply tmc_dps_constr_1; first constructor.
-      * eapply tmc_dps_call; repeat constructor.
+      eapply tmc_expr_dps_constr_1; first constructor.
+      * eapply tmc_expr_dps_call; repeat constructor.
       * done.
 Qed.
